to_node_list_inverse_core 에서 막히네 와;;

src/study/Nemonuri.Study.CSharpSyntaxRewriter2.Modifier2/Nemonuri.StratifiedNodes.Internals.fst
@@ -1,6 +1,7 @@
 module Nemonuri.StratifiedNodes.Internals
 
 module L = FStar.List.Tot
+module Math = FStar.Math.Lib
 
 //--- type definitions ---
 type node_internal (t:eqtype) : pos -> Type =
@@ -17,7 +18,7 @@ and node_list_internal (t:eqtype) : nat -> Type =
       #tl_level:nat ->
       hd:(node_internal t hd_level) ->
       tl:(node_list_internal t tl_level) ->
-      node_list_internal t (if hd_level >= tl_level then hd_level else tl_level)
+      node_list_internal t (Math.max hd_level tl_level)
 //---|
 
 //--- theory members ---
@@ -28,6 +29,42 @@ let rec select
   match nl with
   | SNil -> []
   | SCons #_ #_ hd tl -> (selector hd)::(select tl selector)
+
+let rec contains
+  #t #node_level #max_level
+  (nd:node_internal t node_level) (nl:node_list_internal t max_level)
+  : Tot bool (decreases nl) =
+  match nl with
+  | SNil -> false
+  | SCons #_ #_ hd tl ->
+      if (((SCons?.hd_level nl) = node_level) && (hd = nd)) then true
+      else (contains nd tl)
+//---|
+
+//--- proofs ---
+let rec lemma_select_result_contains_selector_result
+  #t (#t2:eqtype) #node_level #max_level (nl:node_list_internal t max_level)
+  (selector:((#lv:pos) -> node_internal t lv -> Tot t2))
+  (nd:node_internal t node_level) (selector_result:t2)
+  : Lemma (requires (contains nd nl) && ((selector nd) = selector_result))
+          (ensures L.contains selector_result (select nl selector))
+          (decreases nl)
+  = 
+  let select_result = select nl selector in
+  if (((SCons?.hd_level nl) = node_level) && ((SCons?.hd nl) = nd)) then
+    assert ((L.hd select_result) = selector_result)
+  else
+    lemma_select_result_contains_selector_result (SCons?.tl nl) selector nd selector_result
+
+let rec lemma_node_list_internal_level_is_greater_or_equal_than_element_level
+  #t #node_level #max_level
+  (nd:node_internal t node_level) (nl:node_list_internal t max_level)
+  : Lemma (requires contains nd nl)
+          (ensures max_level >= node_level)
+          (decreases nl)
+  =
+  if (((SCons?.hd_level nl) = node_level) && ((SCons?.hd nl) = nd)) then ()
+  else lemma_node_list_internal_level_is_greater_or_equal_than_element_level nd (SCons?.tl nl)
 //---|
 
 
