src/study/Nemonuri.Study.CSharpSyntaxRewriter2.Modifier2/Nemonuri.StratifiedNodes.Nodes.fst
@@ -1,5 +1,7 @@
 module Nemonuri.StratifiedNodes.Nodes
 
+module L = FStar.List.Tot
+module Math = FStar.Math.Lib
 module I = Nemonuri.StratifiedNodes.Internals
 
 //--- type definitions ---
@@ -19,7 +21,7 @@ let to_node #t #level (node_internal:I.node_internal t level) : Tot (node t) =
 let to_node_list #t #max_level 
   (node_list_internal:I.node_list_internal t max_level) 
   : Tot (node_list t) =
-  I.select node_list_internal (fun ni -> to_node ni)
+  I.select node_list_internal (fun ni -> to_node ni)  
 //---|
 
 //--- (node t) members ---
@@ -31,4 +33,112 @@ let get_children #t (node:node t) : Tot (node_list t) =
   to_node_list node.internal.children
 //---|
 
+//--- (node_list t) members ---
+private let rec get_max_core (l:list pos) (seed:pos)
+  : Tot pos (decreases l) =
+  match l with
+  | [] -> seed
+  | hd::tl ->
+      let seed2 = (if hd > seed then hd else seed) in
+      get_max_core tl seed2
+
+private let get_max (l:list pos)
+  : Tot (n:nat{ if L.isEmpty l then n = 0 else n > 0 }) =
+  match l with
+  | [] -> 0
+  | hd::tl -> get_max_core tl hd
+  
+let get_max_level #t (l:node_list t) 
+  : Tot (n:nat{ if L.isEmpty l then n = 0 else n > 0 }) =
+  get_max (L.map (fun nd -> (get_level nd)) l)
+//---|
+
+//--- propositions ---
+//let node_internal_children_and_get_children_result_
+
+let node_level_is_greater_than_levels_of_nodes_in_children 
+  #t (node1:node t) : Tot prop =
+  forall (node2:node t). 
+    (L.contains node2 (get_children node1)) ==> ((get_level node1) > (get_level node2))
+//---|
+
+//--- theory members for proofs ---
+private let to_node_inverse #t (nd:node t) : Tot (I.node_internal t (get_level nd)) =
+  nd.internal
+
+private let rec to_node_list_inverse_core 
+  #t #node_list_internal_level (l:node_list t) (seed:I.node_list_internal t node_list_internal_level)
+  : Tot (I.node_list_internal t (Math.min (get_max_level l) node_list_internal_level))
+        (decreases l)
+  =
+  match l with
+  | [] -> seed
+  | hd::tl ->
+      let seed2 = I.SCons (to_node_inverse hd) seed in
+      to_node_list_inverse_core tl seed2
+
+
+(*
+  : Tot (I.node_list_internal t (
+      match l with
+      | [] -> node_list_internal_level
+      | hd::_ -> Math.max (get_level hd) node_list_internal_level
+    )) 
+    (decreases l)
+*)
+
+(*
+private let rec to_node_list_inverse #t (l:node_list t) 
+  : Tot (I.node_list_internal t (get_max_level l)) 
+        (decreases l)     
+  =
+  match l with
+  | [] -> I.SNil
+  | hd::tl -> 
+      let hd2 = to_node_inverse hd in
+      I.SCons hd2 (to_node_list_inverse tl)
+  //I.SCons 
+*)
+//---|
+
+//--- proofs ---
+open FStar.Classical.Sugar
+
+let lemma_to_node_is_bijection #t
+  : Lemma (ensures forall (lv:pos) (ni:I.node_internal t lv). (to_node_inverse (to_node ni)) = ni)
+  =
+  ()
+
+//let lemma_to_node_
+
+(*
+let lemma_node1_children_contains_node2_entails_node1_internal_children_contains_node2_internal
+  #t (node1:node t) (node2:node t)
+  : Lemma (requires (L.contains node2 (get_children node1)))
+          (ensures (I.contains node2.internal node1.internal.children))
+          
+  =
+  introduce forall (node1:node t) (node2:node t)
+*)
+
+
+let lemma_node_level_is_greater_than_level_of_node_in_children
+  #t (node1:node t) (node2:node t)
+  : Lemma (requires (L.contains node2 (get_children node1)))
+          (ensures ((get_level node1) > (get_level node2)))
+  =
+  assert ((to_node node2.internal) = (node2));
+  assert (I.contains node2.internal node1.internal.children);
+  I.lemma_node_list_internal_level_is_greater_or_equal_than_element_level node2.internal node1.internal.children
+
+
+
+(*
+let lemma_node_level_is_greater_than_levels_of_nodes_in_children
+  #t (node1:node t)
+  : Lemma (ensures node_level_is_greater_than_levels_of_nodes_in_children node1) =
+  introduce forall (node2:node t{L.contains node2 (get_children node1)}). 
+    (I.contains node2.internal node1.internal.children) with ((to_node node2.internal) = (node2))
+*)
+//---|
   
