src/study/Nemonuri.Study.CSharpSyntaxRewriter2.Modifier2/Nemonuri.StratifiedNodes.Children.fst
@@ -1,0 +1,14 @@
+module Nemonuri.StratifiedNodes.Children
+
+module L = FStar.List.Tot
+module N = Nemonuri.StratifiedNodes.Nodes
+
+//--- propositions ---
+
+//---|
+
+let is_child #t (parent_node:N.node t) (node:N.node t) 
+  : Tot (b:bool{if b then (N.get_level node) < (N.get_level parent_node) else true})
+  =
+  L.contains node (N.get_children parent_node)
+
